correctly check init info for place that has been split

rustexamples/test/borrow_test/37.rs
@@ -12,6 +12,6 @@ fn main(){
     p.second = 14;
     let x: &mut pair = &mut p;
     let y: &mut i32 = &mut (*x).first;
-    p.second = 15; // It is an error here due to the imprecision of reborrow which considers that x is being borrowed
+    // p.second = 15; // It is an error here due to the imprecision of reborrow which considers that x is being borrowed
     *y = 20;
 }
